port Assert to Prop as far as possible

theories/Assert.v
@@ -3,24 +3,29 @@ Require Import Setoid.
 Require Import Trace.
 Require Import Language.
 
+Add Relation trace bisim 
+reflexivity proved by bisim_reflexive
+symmetry proved by bisim_symmetric 
+transitivity proved by bisim_transitive
+as bisim_rel.
+
 Set Implicit Arguments.
 Unset Strict Implicit.
 Import Prenex Implicits.
 
-Definition setoid (p: trace -> Type) :=
+Definition setoid (p: trace -> Prop) :=
 forall tr0, p tr0 -> forall tr1, bisim tr0 tr1 -> p tr1.  
-Definition assertS := state -> Type.
-Definition assertT := { p:  trace -> Type & setoid p}.
+Definition assertS := state -> Prop.
+Definition assertT := { p:  trace -> Prop | setoid p}.
 
-Definition assertS_and (u1 u2: assertS) := 
-fun st =>  prod (u1 st) (u2 st).
+Definition assertS_and (u1 u2: assertS) := fun st =>  u1 st /\ u2 st.
 
 Infix "andS" := assertS_and (at level 60, right associativity).
 
 Definition assertT_and0 (p1 p2: assertT) :=
-let: existT f0 h0 := p1 in
-let: existT f1 h1 := p2 in
-fun tr => prod (f0 tr) (f1 tr).  
+let: exist f0 h0 := p1 in
+let: exist f1 h1 := p2 in
+fun tr => f0 tr /\ f1 tr.  
 
 Lemma assertT_and0_setoid: forall p0 p1, setoid (assertT_and0 p0 p1). 
 move => [f0 h0] [f1 h1]. simpl.  
@@ -31,35 +36,37 @@ Qed.
 
 
 Definition assertT_and (p1 p2: assertT): assertT. 
-destruct p1 as [f0 h0]. destruct p2 as [f1 h1]. exists (fun tr => prod (f0 tr) (f1 tr)). 
+destruct p1 as [f0 h0]. 
+destruct p2 as [f1 h1]. exists (fun tr => f0 tr /\ f1 tr). 
 move => tr0 [h2 h3] tr1 h4. split. 
 * have := h0 _ h2 _ h4; apply. 
 * have := h1 _ h3 _ h4; apply.
-Defined.   
+Qed.
 
 Infix "andT" := assertT_and (at level 60, right associativity).
 
 Definition assertT_or (p1 p2: assertT): assertT. 
 destruct p1 as [f0 h0]. 
-destruct p2 as [f1 h1]. 
-exists (fun tr => sum (f0 tr) (f1 tr)). 
+destruct p2 as [f1 h1]. exists (fun tr => f0 tr \/ f1 tr). 
 move => tr0 [h2 | h2] tr1 h3.
 - left. have := h0 _ h2 _ h3; apply. 
 - right. have := h1 _ h2 _ h3; apply. 
-Defined.    
+Defined.
 
-Infix "orT" := assertT_or (at level 60, right associativity). 
+Infix "orT" := assertT_or (at level 60, right associativity).
 
 Definition assertS_imp (u1 u2: assertS) := forall st, u1 st -> u2 st. 
 
 Infix "->>" := assertS_imp (at level 60, right associativity).
 
 Lemma assertS_imp_refl: forall u, u ->> u. 
-Proof. move => u st0 h0. done. Qed. 
+Proof. 
+move => u st0 h0. done. 
+Qed.
 
-Definition satisfy (p:assertT) (tr: trace): Type := 
-let: existT f0 h0 := p in f0 tr.
- 
+Definition satisfy (p:assertT) (tr: trace): Prop := 
+let: exist f0 h0 := p in f0 tr.
+
 Definition assertT_imp (p1 p2: assertT) := 
 forall tr, satisfy p1 tr -> satisfy p2 tr.  
 
@@ -77,40 +84,40 @@ q0 =>> q1 -> p =>> q0 -> p =>> q1.
 Proof. move => p q0 q1. destruct p as [p hp]. 
 destruct q0 as [q0 hq0]. destruct q1 as [q1 hq1]. 
 move => h0 h1 tr0. simpl. move => h2. apply h0. simpl. 
-apply h1. simpl. done. Qed.    
+apply h1. simpl. done. Qed.
 
+Inductive ttS: state -> Prop := | ttS_intro: forall st, ttS st.
+Definition ffS: assertS := fun st => False.
 
-Inductive ttS: state -> Type := | ttS_intro: forall st, ttS st.  
-Definition ffS: assertS := fun st => Empty_set.
-
-Inductive ttt: trace -> Type := | ttt_intro: forall tr, ttt tr.
+Inductive ttt: trace -> Prop := | ttt_intro: forall tr, ttt tr.
 Definition ttT: assertT.
 exists ttt. move => tr0 h0 tr1 h1. apply ttt_intro. 
-Defined.  
+Defined.
 
 Lemma assertT_imp_refl: forall p, p =>> p. 
 Proof. move => p tr0 h0. done. Qed. 
 
-Lemma satisfy_monotone: forall p0 p1, 
+Lemma satisfy_cont: forall p0 p1, 
 p0 =>> p1 -> forall tr, satisfy p0 tr -> satisfy p1 tr. 
 Proof. move => [f0 h0] [f1 h1] h2 tr h3. 
 simpl. simpl in h3. have := h2 _ h3. apply. 
-Qed.   
+Qed.
 
 Lemma assertT_imp_trans: forall p q r, p =>> q -> q =>> r -> p =>> r.
 Proof. 
 move => p q r h0 h1 tr0 h2.  
-have := satisfy_monotone h1. apply. 
-have := satisfy_monotone h0 h2. by apply. 
-Qed.  
-
+have := satisfy_cont h1. apply. 
+have := satisfy_cont h0 h2. by apply. 
+Qed.
 
 Lemma andS_left: forall u1 u2, (u1 andS u2) ->> u1. 
 Proof. move => u1 u2 st h1; by inversion h1. Qed.  
 Lemma andS_right: forall u1 u2, (u1 andS u2) ->> u2.
 Proof. move => u1 u2 st h1; by inversion h1. Qed.   
-Lemma andS_monotone: forall u1 u1' u2 u2',
-u1 ->> u1' -> u2 ->> u2' -> (u1 andS u2) ->> (u1' andS u2').
+Lemma andS_cont: forall u1 u1' u2 u2',
+u1 ->> u1' ->
+u2 ->> u2' ->
+(u1 andS u2) ->> (u1' andS u2').
 Proof. 
 move => u1 u1' u2 u2' h1 h2 st [h3 h4]. split. 
 * have := h1 _ h3; apply. 
@@ -129,37 +136,32 @@ move => p1 p2 tr h1. simpl. destruct p1 as [f1 hf1].
 destruct p2 as [f2 hf2]. simpl. simpl in h1. by right. 
 Qed. 
 
-
-Definition singleton (u:assertS): trace -> Type :=
-fun tr => { st: state & prod (u st) (bisim tr (Tnil st))}.
+Definition singleton (u:assertS): trace -> Prop :=
+fun tr => exists st, u st /\ bisim tr (Tnil st).
 
 Lemma singleton_setoid: forall u, setoid (singleton u). 
 Proof. 
 move => u. move => tr0 h0 tr1 h1. move: h0 => [st0 [h0 h2]]. 
-foo h2. foo h1. exists st0. split; [apply h0 | apply bisim_reflexive]. 
-Qed. 
+foo h2. foo h1. exists st0. split; [apply h0 | reflexivity]. 
+Qed.
 
 Lemma singleton_monotone: forall u v, u ->> v ->
 forall tr, singleton u tr ->  singleton v tr.
 Proof. 
 move => u v huv tr0 h0. move: h0 => [st0 [h0 h1]]. foo h1. 
 exists st0. split; [ have := huv _ h0; apply | apply bisim_reflexive].
-Qed.   
+Qed.
 
 Lemma singleton_nil: forall u st,
 singleton u (Tnil st) -> u st. 
-Proof. move => u st [st0 [h0 h1]]. foo h1. done. Qed.  
-
-Lemma mk_singleton_nil: forall u st,
-u st -> singleton u (Tnil st). 
-Proof. move => u st h0. exists st. split; [ done | apply bisim_reflexive]. Qed. 
+Proof. move => u st [st0 [h0 h1]]. foo h1. done. Qed.
 
 (* Proposition 3.1: <U> is setoid *)
 Definition Singleton (u: assertS): assertT. 
 exists (singleton u). 
 move => tr0 [st0 [h0 h1]] tr1 h2. foo h1. foo h2.
 exists st0. by split; [done | apply bisim_nil]. 
-Defined. 
+Defined.
 
 Notation "[| p |]" := (Singleton p) (at level 80).
 
@@ -169,40 +171,40 @@ u ->> v -> [|u|] =>> [|v|].
 Proof. 
 move => u v h0 tr0 h1. move: h1 => [st0 [h1 h2]]. 
 foo h2. exists st0. split; [ have := h0 _ h1; apply | apply bisim_reflexive].
-Qed.  
+Qed.
 
 Definition eval_true (a: expr): assertS  :=
 fun st => is_true (a st) = true. 
 
 Definition eval_false (a: expr): assertS :=
-fun st => is_true (a st) = false. 
+fun st => is_true (a st) = false.
 
-Definition dup (u: assertS): trace -> Type :=
-fun tr => { st: state & prod (u st) (bisim tr (Tcons st (Tnil st))) }. 
+Definition dup (u: assertS): trace -> Prop :=
+fun tr => exists st, u st /\ bisim tr (Tcons st (Tnil st)).
 
-Lemma dup_monotone: forall (u0 u1: assertS),
+Lemma dup_cont: forall (u0 u1: assertS),
 u0 ->> u1 ->
 forall tr, dup u0 tr -> dup u1 tr. 
 Proof. 
 move => u0 u1 hu tr [st0 [h0 h1]]. foo h1. foo H1. 
-exists st0. split. have := hu _ h0; apply. apply bisim_reflexive.  
-Qed. 
+exists st0. split. have := hu _ h0; apply. reflexivity. 
+Qed.
 
 (* Proposition 3.1: <<U>> is setoid *)
 Definition Dup (u: assertS): assertT. 
 exists (dup u).
 move => tr0 [st0 [h0 h1]] tr1 h2. foo h1. foo H1. foo h2. foo H2. 
-exists st0. split =>//. apply bisim_reflexive.  
-Defined.    
+exists st0. split =>//. reflexivity. 
+Defined.
 
 Notation "<< p >>" := (Dup p) (at level 80).
 
 (* Proposition 3.2: <<U>> is monotone *)
 Lemma Dup_monotone: forall u v, u ->> v -> <<u>> =>> <<v>>.
-Proof. move => u v h0 tr0. simpl. apply dup_monotone => //. 
-Qed.  
+Proof. move => u v h0 tr0. simpl. apply dup_cont => //. 
+Qed.
 
-CoInductive follows (p: trace -> Type): trace -> trace -> Type :=
+CoInductive follows (p: trace -> Prop): trace -> trace -> Prop :=
 | follows_nil: forall st tr,
   hd tr = st -> p tr ->
   follows p (Tnil st) tr 
@@ -215,7 +217,7 @@ Proof.
 move => p tr0 tr1 h0. by foo h0; simpl. 
 Qed.
 
-Lemma follows_setoid: forall (p: trace -> Type)
+Lemma follows_setoid: forall (p: trace -> Prop)
 (hp: forall tr0, p tr0 -> forall tr1, bisim tr0 tr1 -> p tr1), 
 forall tr0 tr1, follows p tr0 tr1 ->
 forall tr2, bisim tr0 tr2 -> forall tr3, bisim tr1 tr3 -> 
@@ -224,21 +226,20 @@ Proof.
 move => p hp. cofix COINDHYP.
 move => tr0 tr1 h0 tr2 h1 tr3 h2. foo h0. 
 - clear COINDHYP. foo h1. have h0 := bisim_hd h2. symmetry in h0. 
-  have := follows_nil h0 (hp _ X _ h2). apply. 
-- foo h2. foo h1. have := follows_delay st (COINDHYP _ _ X _ H3 _ H2); apply. 
+  have := follows_nil h0 (hp _ H0 _ h2). apply. 
+- foo h2. foo h1. have := follows_delay st (COINDHYP _ _ H _ H4 _ H3); apply. 
 Qed.
-
 
 Lemma follows_setoid_L: forall p,
 forall tr0 tr1, follows p tr0 tr1 ->
 forall tr2, bisim tr0 tr2 ->  follows p tr2 tr1. 
 Proof. 
 move => p. cofix COINDHYP. move =>  tr tr0 h0 tr1 h1. foo h0. 
-- foo h1. apply follows_nil. reflexivity. apply X. 
-- foo h1. have := follows_delay st (COINDHYP _ _ X _ H2). apply. 
-Qed. 
+- foo h1. apply follows_nil. reflexivity. apply H0. 
+- foo h1. have := follows_delay st (COINDHYP _ _ H _ H3). apply. 
+Qed.
 
-Lemma follows_setoid_R: forall (p: trace -> Type)
+Lemma follows_setoid_R: forall (p: trace -> Prop)
 (hp: forall tr0, p tr0 -> forall tr1, bisim tr0 tr1 -> p tr1), 
 forall tr tr0, follows p tr tr0 ->
 forall tr1, bisim tr0 tr1 ->  follows p tr tr1. 
@@ -246,17 +247,17 @@ Proof.
 move => p hp. cofix COINDHYP. 
 move => tr tr0 h0 tr1 h1. foo h0.  
 - apply follows_nil. symmetry. have := bisim_hd h1. apply. 
-  have := hp _ X _ h1; apply.  
-- foo h1. have := follows_delay st (COINDHYP _ _  X _ H2). apply.
+  have := hp _ H0 _ h1; apply.  
+- foo h1. have := follows_delay st (COINDHYP _ _  H _ H3). apply.
 Qed.
 
-Lemma follows_monotone: forall p q,
+Lemma follows_monotone: forall (p q : trace -> Prop),
 (forall tr, p tr -> q tr) -> 
 forall tr0 tr1, follows p tr0 tr1 -> follows q tr0 tr1.
 Proof. 
 move => p q hpq. cofix hcoind. move => tr0 tr1 h0. foo h0. 
-- apply follows_nil => //. have := hpq _ X; by apply.
-- have := follows_delay _ (hcoind _ _ X). by apply. 
+- apply follows_nil => //. have := hpq _ H0; by apply.
+- have := follows_delay _ (hcoind _ _ H). by apply. 
 Qed.    
 
 (* Lemma 3.2 *)
@@ -264,8 +265,8 @@ Lemma follows_singleton: forall u tr0 tr1,
 follows (singleton u) tr0 tr1 -> bisim tr0 tr1.
 Proof. 
 move => u. cofix COINDHYP. move => tr0 tr1 h0. foo h0. 
-- simpl in X. move: X => [st0 [h0 h1]]. foo h1. simpl; apply bisim_reflexive.  
-- have := bisim_cons st (COINDHYP _ _ X); apply.
+- move: H0 => [st0 [h0 h1]]. foo h1. by simpl; apply bisim_reflexive.  
+- have := bisim_cons st (COINDHYP _ _ H); apply.
 Qed.
 
 Lemma follows_singleton_andS_L: forall u0 u1 tr0,
@@ -273,11 +274,12 @@ follows (singleton (u0 andS u1)) tr0 tr0 ->
 follows (singleton u0) tr0 tr0.
 Proof. 
 move => u0 u1. cofix hcoind. case. 
-- move => st0 h0. inversion h0. clear H1 H. simpl in H0. 
-  move: X => [st1 [h1 h2]]. foo h2. move: h1 => [h1 h2].
+- move => st0 h0. inversion h0. clear H1 H. simpl in H0.
+  foo h0.
+  move: H3 => [st1 [h1 h2]]. foo h2. move: h1 => [h1 h2].
   apply follows_nil => //. exists st1. split; [done | apply bisim_reflexive].
 - move => st0 tr0 h0. foo h0. 
-  have := follows_delay st0 (hcoind _ X). by apply. 
+  have := follows_delay st0 (hcoind _ H0). by apply. 
 Qed. 
 
 Lemma follows_singleton_andS_R: forall u0 u1 tr0,
@@ -285,22 +287,25 @@ follows (singleton (u0 andS u1)) tr0 tr0 ->
 follows (singleton u1) tr0 tr0.
 Proof. 
 move => u0 u1. cofix hcoind. case. 
-- move => st0 h0. inversion h0. clear H1 H. simpl in H0. 
-  move: X => [st1 [h1 h2]]. foo h2. move: h1 => [h1 h2].
+- move => st0 h0. inversion h0. clear H1 H. simpl in H0.
+  foo h0.
+  move: H3 => [st1 [h1 h2]]. foo h2. move: h1 => [h1 h2].
   apply follows_nil => //. exists st1. split; [done | apply bisim_reflexive].
 - move => st0 tr0 h0. foo h0. 
-  have := follows_delay st0 (hcoind _ X). by apply. 
+  have := follows_delay st0 (hcoind _ H0). by apply. 
 Qed. 
      
 Lemma singleton_andS_follows: forall u v tr,
 follows (singleton u) tr tr -> follows (singleton v) tr tr ->
 follows (singleton (u andS v)) tr tr. 
 Proof. 
-move => u v. cofix hcoind. move => tr h0 h1. inversion h0. 
+move => u v. cofix hcoind. move => tr h0 h1. inversion h0; subst.
 - apply follows_nil => //. exists st. split; last by apply bisim_reflexive. 
-  clear H H1. subst. inversion h1. clear H0 H1. subst. 
-  split; [ have := singleton_nil X; apply | have := singleton_nil X0; apply]. 
-- subst. foo h0. foo h1. have := follows_delay st (hcoind _ X0 X1); by apply. 
+  clear H. inversion h1; subst. clear H1.
+  have := singleton_nil H0.
+  have := singleton_nil H2.
+  by split.
+- subst. foo h0. foo h1. have := follows_delay st (hcoind _ H1 H2); by apply. 
 Qed.  
 
 CoFixpoint lastdup (tr: trace): trace :=
@@ -314,25 +319,25 @@ Proof.
 case. 
 - move => st. rewrite [lastdup _]trace_destr. by simpl.
 - move => st tr. rewrite [lastdup _]trace_destr. by simpl.
-Qed.   
+Qed.
 
 Lemma follows_dup: forall u tr, follows (singleton u) tr tr ->
 follows (dup u) tr (lastdup tr). 
 Proof.
 move => u. cofix COINDHYP. move => tr0 h0. inversion h0. 
-- clear h0 H H0 H1. rewrite [lastdup _]trace_destr. simpl. 
-  move: X => [st1 [h0 h1]]. foo h1. apply follows_nil => //. exists st1.
-  split; [done | apply bisim_reflexive]. 
-- clear h0 H H1. rewrite [lastdup _]trace_destr. simpl. 
-  have := follows_delay st (COINDHYP _ X). apply. 
+- clear H H1 H2 h0. rewrite [lastdup _]trace_destr. simpl. 
+  move: H0 => [st1 [h0 h1]]. foo h1. apply follows_nil => //. exists st1.
+  split; [done | reflexivity]. 
+- clear h0 H0 H. rewrite [lastdup _]trace_destr. simpl. 
+  have := follows_delay st (COINDHYP _ H1). apply. 
 Qed.
 
-Definition append (p1 p2: trace -> Type): trace -> Type :=
-fun tr => { tr': trace &  prod (p1 tr') (follows p2 tr' tr) }.
+Definition append (p1 p2: trace -> Prop ): trace -> Prop :=
+fun tr => exists tr', p1 tr' /\ follows p2 tr' tr.
 
 Infix "*+*" := append (at level 60, right associativity).
 
-Lemma append_monotone: forall (p0 p1 q0 q1: trace -> Type),
+Lemma append_cont: forall (p0 p1 q0 q1: trace -> Prop),
 (forall tr, p0 tr -> p1 tr) ->
 (forall tr, q0 tr -> q1 tr) ->
 forall tr, append p0 q0 tr -> append p1 q1 tr. 
@@ -341,32 +346,32 @@ move => p0 p1 q0 q1 hp hq tr [tr0 [h0 h1]].
 exists tr0. split. have := hp _ h0; apply. clear h0. 
 move: tr0 tr h1. cofix COINDHYP. 
 move => tr0 tr1 h0. foo h0.
-- apply follows_nil => //. have := hq _ X; apply. 
-- have := follows_delay st (COINDHYP _ _ X); apply. 
-Qed.    
+- apply follows_nil => //. have := hq _ H0; apply. 
+- have := follows_delay st (COINDHYP _ _ H); apply. 
+Qed.
 
-Lemma append_monotone_L: forall (p0 p1 q: trace -> Type),
+Lemma append_cont_L: forall (p0 p1 q: trace -> Prop),
 (forall tr, p0 tr -> p1 tr) ->
 forall tr, (append p0 q tr) -> (append p1 q tr).
 Proof. 
 move => p0 p1 q hp. move => tr [tr0 [h0 h1]]. 
 exists tr0. split. have := hp _ h0; apply. apply h1. 
-Qed.  
+Qed.
 
-Lemma append_monotone_R: forall (p q0 q1: trace -> Type),
+Lemma append_monotone_R: forall (p q0 q1: trace -> Prop),
 (forall tr, q0 tr -> q1 tr) ->
 forall tr, (append p q0 tr) -> (append p q1 tr).
 Proof. 
-move => p q0 q1 hq. have := (@append_monotone p p _ _ _ hq). apply => //.    
-Qed.  
+move => p q0 q1 hq. have := (@append_cont p p _ _ _ hq). apply => //.
+Qed.
 
-Lemma append_setoid: forall (p0 p1: trace -> Type),
+Lemma append_setoid: forall (p0 p1: trace -> Prop),
 setoid p1 -> setoid (append p0 p1). 
 Proof. 
 move => p0 p1 hp1. move => tr0 h0 tr1 h1.
 move: h0 => [tr2 [h0 h2]]. exists tr2. split; first by apply h0.
 have := follows_setoid_R hp1 h2 h1. apply. 
-Qed.  
+Qed.
 
 Lemma follows_follows: forall p q tr0 tr1 tr2, follows p tr0 tr1 ->
 follows q tr1 tr2 -> follows (p *+* q) tr0 tr2. 
@@ -374,9 +379,10 @@ Proof. move => p q. cofix hcoind. case.
 - move => st0 tr1 tr2 h0 h1. foo h0. have := follows_hd h1 => h2. 
   apply follows_nil => //. exists tr1. split => //. 
 - move => st0 tr0 tr1 tr2 h0 h1. foo h0. foo h1. apply follows_delay. 
-  have := hcoind _ _ _ X X0. apply.
-Qed.    
+  have := hcoind _ _ _ H2 H3. apply.
+Qed.
 
+(*
 CoFixpoint midp (p0 p1: trace -> Type)  (tr0 tr1: trace) (h: follows (append p0 p1) tr0 tr1): trace :=
 match h with
 | follows_nil _ _ _ h1 => let: existT tr2 h2 := h1 in tr2
@@ -413,7 +419,7 @@ apply follows_nil. by simpl. apply X.
 subst. by apply f. 
 subst. rewrite [midp _]trace_destr. simpl. apply follows_delay. 
 have := COINDHYP _ _ _ _ f; apply. 
-Qed.    
+Qed.
  
 
 Lemma append_assoc_R: forall p1 p2 p3,
@@ -437,43 +443,45 @@ move: tr2 tr0 tr1 h2 h3. cofix COINDHYP. move => tr0 tr1 tr2 h1 h2. foo h2.
   exists tr2. by split. 
 - foo h1. apply follows_delay. have := COINDHYP _ _ _ X0 X; apply. 
 Qed. 
+*)
 
 (* Proposition 3.1: ** is setoid. *)
 Definition Append (p1 p2: assertT): assertT.  
 destruct p1 as [f0 h0]. 
-destruct p2 as [f1 h1]. 
-exists (append f0 f1).  
+destruct p2 as [f1 h1]. exists (append f0 f1).  
 move => tr0 [tr1 [h2 h3]] tr2 h4. exists tr1.
 split. apply h2.  have := follows_setoid_R h1 h3 h4. apply.  
-Defined.   
+Defined. 
 
 Infix "***" := Append (at level 60, right associativity).
 
 
 (* Lemma 3.4 (4) <= *)
+(*
 Lemma Append_assoc_R: forall p1 p2 p3,
 (p1 *** p2 *** p3) =>> (p1 *** p2) *** p3.
 Proof. 
 move => p1 p2 p3 tr0 h1. destruct p1 as [f1 hf1]. destruct p2 as [f2 hf2]. 
 destruct p3 as [f3 hf3]. simpl. simpl in h1. apply append_assoc_R. by apply h1. 
 Qed. 
+*)
 
 (* Lemma 3.4 (4) => *)
+(*
 Lemma Append_assoc_L: forall p1 p2 p3,
 ((p1 *** p2) *** p3) =>> (p1 *** p2 *** p3).
 Proof. 
 move => p1 p2 p3 tr0 h1. destruct p1 as [f1 hf1]. destruct p2 as [f2 hf2]. 
 destruct p3 as [f3 hf3]. simpl. simpl in h1. have := append_assoc_L h1. apply. 
 Qed.
-
-
+*)
 
 (* Proposition 3.2: ** is monotone *)
 Lemma Append_monotone: forall p1 p2 q1 q2,
 p1 =>> p2 -> q1 =>> q2 -> (p1 *** q1) =>> (p2 *** q2). 
 Proof. move => p1 p2 q1 q2 h0 h1. destruct p1 as [p1 hp1]. destruct p2 as [p2 hp2].
 destruct q1 as [q1 hq1]. destruct q2 as [q2 hq2].  move => tr0. simpl. 
-move => h2. have := append_monotone _ _ h2. apply. apply h0. apply h1. 
+move => h2. have := append_cont _ _ h2. apply. apply h0. apply h1. 
 Qed.   
 
 Lemma Append_monotone_L: forall p1 p2 q,
@@ -481,7 +489,7 @@ p1 =>> p2 -> (p1 *** q) =>> (p2 *** q).
 Proof. 
 move => p1 p2 q h0. destruct p1 as [p1 hp1]. destruct p2 as [p2 hp2].
 destruct q as [q hq]. move => tr0. simpl.  
-have := append_monotone_L h0.  apply.
+have := append_cont_L h0.  apply.
 Qed.   
 
 Lemma Append_monotone_R: forall q p1 p2,
@@ -489,14 +497,14 @@ p1 =>> p2 -> (q *** p1) =>> (q *** p2).
 Proof. 
 move => q p1 p2 h0. destruct p1 as [p1 hp1]. destruct p2 as [p2 hp2].
 destruct q as [q hq]. move => tr0. simpl. move => h1.   
-have := (@append_monotone q q p1 p2). apply. done. apply h0. 
+have := (@append_cont q q p1 p2). apply. done. apply h0. 
 exact h1.
 Qed.    
 
 (* Lemma 3.4 (1), the first => *)
 Lemma Sglt_Dup_1: forall u v, ([|u|] *** <<v>>) =>> <<u andS v>>.
 Proof. move => u v tr0 [tr1 [h0 h1]]. simpl. destruct h0 as [st0 [h0 h2]]. foo h2. 
-foo h1. destruct X as [st0 [h1 h2]]. foo h2. foo H1. simpl in h0. exists st0. 
+foo h1. destruct H1 as [st0 [h1 h2]]. foo h2. foo H1. simpl in h0. exists st0. 
 split; last by apply bisim_reflexive. by split. Qed. 
 
 (* Lemma 3.4 (1), the first <= *)
@@ -516,14 +524,14 @@ Qed.
 (* Lemma 3.4 (1), the second <= *)
 Lemma Sglt_Dup_4: forall u v, (<<u>> *** [|v|]) =>> <<u andS v>>.
 Proof. move => u v tr0 [tr1 [h0 h1]]. destruct h0 as [st0 [hu h0]]. foo h0. foo H1. 
-foo h1. foo X. destruct X0 as [st0 [hv h0]]. foo h0. simpl in hu. simpl. 
+foo h1. foo H2. destruct H1 as [st0 [hv h0]]. foo h0. simpl in hu. simpl. 
 exists st0. by split; last apply bisim_reflexive. 
 Qed.       
 
 (* Lemma 3.4 (2), => *)
 Lemma Sglt_Chop_1: forall u v, ([|u|] *** [|v|]) =>> [|u andS v|]. 
 Proof. move => u v tr0 [tr1 [h0 h1]]. destruct h0 as [st0 [hu h0]]. foo h0. 
-foo h1. destruct X as [st0 [hv h0]]. foo h0. simpl in hu. exists st0. 
+foo h1. destruct H1 as [st0 [hv h0]]. foo h0. simpl in hu. exists st0. 
 by split; last apply bisim_reflexive. Qed. 
 
 (* Lemma 3.4 (2), <= *)
@@ -534,7 +542,7 @@ exists st0. by split; last apply bisim_reflexive. Qed.
 
 Lemma Singleton_Append: forall v p, ([|v|] *** p) =>> p. 
 Proof. move => v [p hp] tr0. simpl. move => [tr1 [h0 h1]]. 
-destruct h0 as [st0 [h0 h2]]. foo h2. foo h1. done. Qed.     
+destruct h0 as [st0 [h0 h2]]. foo h2. foo h1. done. Qed.
 
 (* Lemma 3.4 (3), the first => *)
 Lemma ttS_Chop: forall p,
@@ -573,11 +581,9 @@ Qed.
 Lemma ttT_idem_comp: (ttT *** ttT) =>> ttT. 
 Proof.
 move => tr _. done. 
-Qed.    
+Qed.
 
-
-
-Inductive finite: trace -> Type :=
+Inductive finite: trace -> Prop :=
 | finite_nil: forall st, finite (Tnil st)
 | finite_delay: forall st tr,
   finite tr -> finite (Tcons st tr).
@@ -615,9 +621,8 @@ move: h0 => [tr1 [h0 h1]].
 have h2 := follows_singleton h1 => {h1}.
 have := finite_setoid h0 h2. by apply. 
 Qed.    
-    
 
-CoInductive iter (p: trace -> Type): trace -> Type :=
+CoInductive iter (p: trace -> Prop): trace -> Prop :=
 | iter_stop: forall st, iter p (Tnil st)
 | iter_loop: forall tr tr0, 
   p tr ->
@@ -630,83 +635,81 @@ move => p hp. cofix COINDHYP.
 have h0: forall tr, setoid (follows (iter p) tr).
 * cofix COINDHYP1. move => tr. move => tr0 h0 tr1 h1. foo h0. 
   - apply follows_nil. symmetry. have := bisim_hd h1. apply. 
-    have := COINDHYP _ X _ h1. apply.  
-  - foo h1. have := follows_delay st (COINDHYP1 _ _ X _ H2). apply.
+    have := COINDHYP _ H0 _ h1. apply.  
+  - foo h1. have := follows_delay st (COINDHYP1 _ _ H _ H3). apply.
 * move => tr0 h1 tr1 h2. foo h1. 
   - foo h2. apply iter_stop. 
-  - have := iter_loop X (h0 _ _ X0 _ h2). apply. 
-Qed. 
+  - have := iter_loop H (h0 _ _ H0 _ h2). apply. 
+Qed.
 
-Lemma iter_cont: forall (p0 p1: trace -> Type),
+Lemma iter_cont: forall (p0 p1: trace -> Prop),
 (forall tr, p0 tr -> p1 tr) ->
 forall tr, iter p0 tr -> iter p1 tr. 
 Proof. 
 move => p0 p1 hp. cofix COINDHYP. 
 have h: forall tr0 tr1, follows (iter p0) tr0 tr1 -> follows (iter p1) tr0 tr1.
 * cofix COINDHYP0. move => tr0 tr1 h0. foo h0. 
-  - apply follows_nil. reflexivity. have := COINDHYP _ X; apply. 
-  - have := follows_delay st (COINDHYP0 _ _ X). apply. 
+  - apply follows_nil. reflexivity. have := COINDHYP _ H0; apply. 
+  - have := follows_delay st (COINDHYP0 _ _ H). apply. 
 * move => tr0 h0. foo h0. 
   - apply iter_stop. 
-  - have := iter_loop (hp _ X)  (h _ _ X0). apply. 
-Qed.  
+  - have := iter_loop (hp _ H)  (h _ _ H0). apply. 
+Qed.
 
-
-Lemma iter_append_dup: forall u p tr,
+Lemma iter_append_dup: forall (u : state -> Prop) p tr,
 u (hd tr) -> iter (append p (dup u)) tr ->
 follows (singleton u) tr tr. 
 Proof. 
 move => u p.  cofix hcoind. move => tr h0 h1. foo h1. 
 - simpl in h0. apply follows_nil => //. exists st. 
   by split; [done | apply bisim_reflexive]. 
-- move: X => [tr1 [h2 h1]]. clear h2 h0. (*
+- move: H => [tr1 [h2 h1]]. clear h2 h0. (*
   have h2 := follows_hd X0.  rewrite -h2 in h0 => {h2}.   *)
-  move: tr tr1 tr0 h1 X0. cofix hcoind1. 
+  move: tr tr1 tr0 h1 H0. cofix hcoind1. 
   move => tr0 tr1 tr2 h0 h1. foo h0.
-  - move: X => [st0 [h0 h3]]. foo h3. foo H1. 
-    foo h1. foo X. have := follows_delay _ (hcoind _ h0 X0). by apply.  
-  - foo h1. have := follows_delay _ (hcoind1 _ _ _ X X0). by apply. 
+  - move: H0 => [st0 [h0 h3]]. foo h3. foo H1. 
+    foo h1. foo H2. have := follows_delay _ (hcoind _ h0 H1). by apply.  
+  - foo h1. have := follows_delay _ (hcoind1 _ _ _ H H3). by apply. 
 Qed. 
-
 
 (* Proposition 3.2: Iter is setoid. *)
 Definition Iter (p: assertT): assertT. 
 destruct p as [f0 h0].  exists (iter f0). apply iter_setoid. apply h0. 
-Defined.  
+Defined.
 
 (* Proposition 3.2: Iter is monotone. *)
 Lemma Iter_monotone: forall p q, p =>> q -> (Iter p) =>> (Iter q). 
 Proof. move => p q h0 tr0. destruct p as [p hp]. destruct q as [q hq]. 
-simpl. apply iter_cont. move => tr1. apply h0. Qed.  
- 
-Definition updt (u: assertS) (x:id) (a: expr): trace -> Type := 
-fun tr => { st: state & prod (u st) (bisim tr (Tcons st (Tnil (update x (a st) st))))}.
+simpl. apply iter_cont. move => tr1. apply h0. Qed.
+
+Definition updt (u: assertS) (x:id) (a: expr): trace -> Prop := 
+fun tr => exists st, u st /\ bisim tr (Tcons st (Tnil (update x (a st) st))).
 
 (* Proposition 3.1: U[x↦e] is setoid. *)
 Definition Updt (u: assertS) (x:id) (a: expr): assertT. 
 exists (updt u x a). 
 move => tr0 [st0 [h0 h1]] tr1 h2. 
 exists st0. foo h1. foo H1. foo h2. foo H2. 
-split; [done | apply bisim_reflexive]. 
-Defined.  
+split; [done | reflexivity]. 
+Defined.
 
 Definition exS (A: Set) (u: A -> assertS): assertS :=
-fun st => { x: A & u x st}.  
+fun st => exists x, u x st.
 
 Definition exT (A: Set) (p: A -> assertT): assertT. 
-exists (fun tr => { x: A & satisfy (p x) tr}).
+exists (fun tr => exists x, satisfy (p x) tr).
 move => tr0 [x h0] tr1 h1. exists x. destruct (p x) as [f0 h2]. 
 simpl. simpl in h0. have := h2 _ h0 _ h1; apply. 
 Defined.
 
 Definition negT (p: assertT): assertT. 
 destruct p as [f hf]. 
-exists (fun tr => f tr -> Empty_set).
+exists (fun tr => f tr -> False).
 move => tr0 h0 tr1 h1. simpl. move => h2. 
 have := hf _ h2 _ (bisim_symmetric h1). apply h0.
 Defined.      
 
-CoInductive infinite: trace -> Set :=
+CoInductive infinite: trace -> Prop :=
 | infinite_delay: forall st tr,
   infinite tr -> infinite (Tcons st tr). 
 
@@ -731,14 +734,12 @@ Lemma true_chop_false_implies_infinite: (ttT *** [|ffS|]) =>> Infinite.
 Proof. 
 move => tr0 [tr1 [_ h1]]. simpl. move: tr0 tr1 h1. cofix h0. move => tr0 tr1 h1. 
 inversion h1; subst; clear h1. 
-- destruct X as [st0 [h1 h2]]. inversion h1. 
-- apply infinite_delay. apply (h0 _ _ X). 
+- destruct H0 as [st0 [h1 h2]]. inversion h1. 
+- apply infinite_delay. apply (h0 _ _ H). 
 Qed. 
 
-
-
 (* extensions *)
-Lemma iter_split_1: forall p tr, iter p tr -> sum (singleton ttS tr) (append p (iter p) tr).
+Lemma iter_split_1: forall p tr, iter p tr -> (singleton ttS tr) \/ (append p (iter p) tr).
 Proof. 
 move => p tr h0. foo h0. 
 - left. exists st. split => //. by apply bisim_reflexive.
@@ -750,11 +751,11 @@ Lemma Iter_unfold_0: forall p, Iter p =>> ([|ttS|] orT (p *** Iter p)).
 Proof. move => [p hp] tr0; simpl => h0. have := iter_split_1 h0. 
 by apply. Qed.
 
-Lemma iter_split_2: forall tr p, sum (singleton ttS tr) (append p (iter p) tr) -> iter p tr. 
+Lemma iter_split_2: forall tr p, (singleton ttS tr) \/ (append p (iter p) tr) -> iter p tr. 
 Proof. 
 move => tr p h. foo h. 
-- move: X => [st [h0 h1]]. foo h1.  apply iter_stop.
-- move: X => [tr0 [h0 h1]]. have := iter_loop h0 h1. by apply. 
+- move: H => [st [h0 h1]]. foo h1.  apply iter_stop.
+- move: H => [tr0 [h0 h1]]. have := iter_loop h0 h1. by apply. 
 Qed.      
 
 (* Lemma 3.4 (5), <= *)
@@ -764,14 +765,14 @@ Proof. move => [p hp] tr0; simpl. apply iter_split_2. Qed.
 Lemma iter_unfold_1: forall p tr, (iter p *+* p) tr -> iter p tr.
 Proof. move => p tr h0.  move: h0 => [tr0 [h0 h1]].
 move: tr0 tr h0 h1. cofix hcoind. move => tr0 tr1 h0 h1. foo h0. 
-- foo h1. have := iter_loop X. apply. clear X. move: tr1. cofix hcoind0. 
+- foo h1. have := iter_loop H1. apply. clear H1. move: tr1. cofix hcoind0. 
   case. move => st. apply follows_nil => //. apply iter_stop. 
   move => st0 tr0. have := follows_delay _ (hcoind0 _). by apply. 
-- have := iter_loop X. apply. clear X. move: tr tr0 tr1 X0 h1.
+- have := iter_loop H. apply. clear H. move: tr tr0 tr1 H0 h1.
   cofix hcoind0. move => tr0 tr1 tr2 h0 h1. foo h0.
   - have h0 := follows_hd h1. apply follows_nil => //. 
-    have := hcoind _ _ X h1. by apply. 
-  - foo h1. have := follows_delay _ (hcoind0 _ _ _ X X0). by apply. 
+    have := hcoind _ _ H0 h1. by apply. 
+  - foo h1. have := follows_delay _ (hcoind0 _ _ _ H H3). by apply. 
 Qed.            
 
 Lemma Iter_unfold_1: forall p, (Iter p *** p) =>> Iter p. 
@@ -783,8 +784,8 @@ have := iter_unfold_1 h0. by apply. Qed.
 (* *)
 Lemma Iter_unfold_2: forall p, ([|ttS|] orT (Iter p *** p)) =>> Iter p. 
 Proof. move => [p hp] tr0; simpl => h0. foo h0. 
-- destruct X as [st0 [_ h0]]. foo h0. by apply iter_stop. 
-- have := iter_unfold_1 X. by apply. 
+- destruct H as [st0 [_ h0]]. foo h0. by apply iter_stop. 
+- have := iter_unfold_1 H. by apply. 
 Qed. 
 
 Lemma Stop_Iter: forall p, [|ttS|] =>> Iter p.
@@ -809,11 +810,11 @@ Lemma iter_iter: forall p tr, append (iter p) (iter p) tr -> (iter p) tr.
 Proof. move => p tr0 [tr1 [h0 h1]]. move: tr1 tr0 h0 h1. cofix hcoind. 
 move => tr0 tr1 h0. foo h0. 
 - move => h0. foo h0. done. 
-- move => h0. have := iter_loop X. apply. clear X. move: tr tr0 tr1 X0 h0. 
+- move => h0. have := iter_loop H. apply. clear H. move: tr tr0 tr1 H0 h0. 
   cofix hcoind2. move => tr0 tr1 tr2 h0. foo h0. 
   - move => h0. have h1 := follows_hd h0. apply follows_nil. done. 
-    have := hcoind _ _ X h0. done. 
-  - move => h0. foo h0. apply follows_delay.  have := hcoind2 _ _ _ X X0. 
+    have := hcoind _ _ H0 h0. done. 
+  - move => h0. foo h0. apply follows_delay.  have := hcoind2 _ _ _ H H3. 
     done. 
 Qed.                   
 
@@ -829,16 +830,11 @@ Proof. cofix hcoind. case.
 - move => st0 tr0. have := follows_delay _ (hcoind _). apply.  
 Qed.       
 
-
-
-
-Inductive fin: trace -> state -> Type :=
+Inductive fin: trace -> state -> Prop :=
 | fin_nil: forall st, fin (Tnil st) st
 | fin_delay: forall st st' tr, fin tr st' -> fin (Tcons st tr) st'.
 
-
-
-Lemma append_fin: forall p q tr0 tr1, p tr0 -> q tr1 -> fin tr0 (hd tr1) ->
+Lemma append_fin: forall (p q : trace -> Prop) tr0 tr1, p tr0 -> q tr1 -> fin tr0 (hd tr1) ->
 (p *+* q) (tr0 +++ tr1). 
 Proof. move => p q tr0 tr1 hp hq hfin. exists tr0. split => //.
 clear hp. move: tr0 tr1 hq hfin. cofix hcoind. case. 
@@ -847,16 +843,16 @@ clear hp. move: tr0 tr1 hq hfin. cofix hcoind. case.
   simpl. apply follows_delay. have := hcoind _ _ h0 H2. done.
 Qed.    
 
-Definition last (p: trace -> Type): assertS := 
-fun st => {tr: trace & prod (p tr) (fin tr st)}.
+Definition last (p: trace -> Prop): assertS := 
+fun st => exists tr, (p tr) /\ (fin tr st).
 
-Lemma last_cont: forall (p q: trace -> Type),
+Lemma last_cont: forall (p q: trace -> Prop),
 (forall tr, p tr -> q tr) ->
 last p ->> last q.
 Proof. 
 move => p0 p1 hp. move => st [tr [h0 h1]]. 
 exists tr. split. have := hp _ h0; apply. apply h1. 
-Qed.     
+Qed.
 
 Definition Last (p: assertT): assertS. 
 destruct p as  [f0 h0]. apply (last f0).
@@ -894,7 +890,7 @@ move: tr0 st h1 tr h2. induction 1.
 - move => tr0 h0. foo h0. exists (Tnil st). split => //. by apply fin_nil. 
 - move => tr0 h0. foo h0.
   - exists (Tcons st tr). split => //. have := fin_delay _ h1. by apply.
-  - have := IHh1 _ X. by apply.
+  - have := IHh1 _ H1. by apply.
 Qed.
 
 (* Lemma 3.4, (13) *)
@@ -903,10 +899,10 @@ Last (p *** [|v|]) ->> v.
 Proof. 
 move => [p hp] v. simpl. move => st [tr [[tr' [_ h0]] h1]].
 move: tr st h1 tr' h0. induction 1. 
-- move => tr0 h0. foo h0. move: X => [st0 [h0 h1]]. by foo h1.
+- move => tr0 h0. foo h0. move: H0 => [st0 [h0 h1]]. by foo h1.
 - move => tr0 h0. foo h0. 
-  - move: X => [st0 [_ h0]]. foo h0. 
-  - have := IHh1 _ X. by apply.
+  - move: H0 => [st0 [_ h0]]. foo h0. 
+  - have := IHh1 _ H1. by apply.
 Qed. 
 
 Lemma Last_andS: forall p u, ((Last p) andS u) ->> Last (p *** [|u|]). 
@@ -921,15 +917,15 @@ Lemma iter_last: forall v,
 ([|v|] *** (Iter (ttT *** Dup v))) =>> (ttT *** [|v|]).
 Proof. 
 move => v. move => tr0 [tr1 [h0 h1]]. move: h0 => [st0 [h0 h2]]. foo h2.
-foo h1. simpl. exists tr0. split => //. move: tr0 h0 X. cofix hcoind. 
+foo h1. simpl. exists tr0. split => //. move: tr0 h0 H1. cofix hcoind. 
 move => tr0 h0 h1. foo h1. 
 - apply follows_nil => //. simpl in h0. exists st. split => //.
   apply bisim_nil. 
-- clear h0. move: X => [tr1 [_ h1]]. move: tr1 tr tr0 h1 X0. cofix hcoind0.
+- clear h0. move: H => [tr1 [_ h1]]. move: tr1 tr tr0 h1 H0. cofix hcoind0.
   move => tr0 tr1 tr2 h0 h1. foo h0. 
-  - move: X => [st0 [h0 h2]]. foo h2. foo H1. foo h1. foo X. 
-    have := follows_delay _ (hcoind _ h0 X0). by apply.   
-  - foo h1. have := follows_delay _ (hcoind0 _ _ _ X X0). apply.
+  - move: H0 => [st0 [h0 h2]]. foo h2. foo H1. foo h1. foo H2. 
+    have := follows_delay _ (hcoind _ h0 H1). by apply.   
+  - foo h1. have := follows_delay _ (hcoind0 _ _ _ H H3). apply.
 Qed. 
 
 (* Lemma 3.4, (14) *)
@@ -947,16 +943,16 @@ Lemma iter_last_dup: forall v,
 (<<v>> *** (Iter (ttT *** <<v>>))) =>> (ttT *** [|v|]).
 Proof. 
 move => v. move => tr0 [tr1 [h0 h1]]. move: h0 => [st0 [h0 h2]]. foo h2.
-foo H1. foo h1. foo X. simpl. exists (Tcons (hd tr') tr'). split => //.
-apply follows_delay => //. move: tr' h0 X0. cofix hcoind. 
+foo H1. foo h1. foo H2. simpl. exists (Tcons (hd tr') tr'). split => //.
+apply follows_delay => //. move: tr' h0 H1. cofix hcoind. 
 move => tr0 h0 h1. foo h1. 
 - apply follows_nil => //. simpl in h0. exists st. split => //.
   apply bisim_nil. 
-- clear h0. move: X => [tr1 [_ h1]]. move: tr1 tr tr0 h1 X0. cofix hcoind0.
+- clear h0. move: H => [tr1 [_ h1]]. move: tr1 tr tr0 h1 H0. cofix hcoind0.
   move => tr0 tr1 tr2 h0 h1. foo h0. 
-  - move: X => [st0 [h0 h2]]. foo h2. foo H1. foo h1. foo X. 
-    have := follows_delay _ (hcoind _ h0 X0). by apply.   
-  - foo h1. have := follows_delay _ (hcoind0 _ _ _ X X0). apply.
+  - move: H0 => [st0 [h0 h2]]. foo h2. foo H1. foo h1. foo H2. 
+    have := follows_delay _ (hcoind _ h0 H1). by apply.   
+  - foo h1. have := follows_delay _ (hcoind0 _ _ _ H H3). apply.
 Qed. 
 
 
@@ -973,8 +969,8 @@ exists (tr2 +++ tr1). split.
   - move => st1 h0. rewrite trace_append_nil. 
     apply follows_nil => //. by foo h0. 
   - move => st1 tr0 h0. foo h0. rewrite trace_append_cons. 
-    apply follows_delay. have := hcoind _ H2. by apply. 
-* clear X h0. move h0: (hd tr1) => st1. rewrite h0 in h2. 
+    apply follows_delay. have := hcoind _ H3. by apply. 
+* clear H1 h0. move h0: (hd tr1) => st1. rewrite h0 in h2. 
   move: tr2 st1 h2 tr1 h0 h1. induction 1. 
   - move => tr0 h0 h1. rewrite trace_append_nil. done. 
   - move => tr0 h0 h1. rewrite trace_append_cons. apply fin_delay. 
